Move implementation of variant into holSyntaxExtraTheory
The motivation here is to make it easier to EVAL the inference system.
The definitions of INST and VSUBST call VARIANT which doesn't have an
EVAL-able definition. But the monadic functions included an
implementation of variant that is obviously evaluatable, and was proved
equivalent.

I have moved the definition of variant (and its dependencies) and its
relevant correctness proofs into holSyntaxExtraTheory, and used them to
provide alternative theorems for INST and VSUBST that will work better
with EVAL.

The theorem for INST is not perfect because it has a precondition
requiring the term argument to be welltyped (and thus cannot be used
directly with EVAL). However, in contexts where welltypedness is known,
it can be used to substitute calls to INST with calls to an alternative
function using the new equations (not defined in this commit).

hol-light/standard/syntax/holSyntaxExtraScript.sml
@@ -42,6 +42,15 @@ val LLEX_EL_THM = store_thm("LLEX_EL_THM",
     Q.EXISTS_TAC`SUC n` THEN SRW_TAC[][] ) THEN
   Cases_on`n` THEN FULL_SIMP_TAC(srw_ss())[] THEN
   METIS_TAC[])
+
+local open pred_setTheory in
+val SUM_SET_IN_LT = store_thm("SUM_SET_IN_LT",
+  ``∀s x y. FINITE s ∧ x ∈ s ∧ y < x ⇒ y < SUM_SET s``,
+  simp[GSYM AND_IMP_INTRO,RIGHT_FORALL_IMP_THM] >>
+  ho_match_mp_tac FINITE_INDUCT >> simp[] >>
+  simp[SUM_SET_THM] >> rw[] >> simp[] >>
+  res_tac >> simp[SUM_SET_DELETE])
+end
 (* -- *)
 
 val type_ind = save_thm("type_ind",
@@ -2297,6 +2306,214 @@ val fresh_term_def = new_specification("fresh_term_def",["fresh_term"],
       match_mp_tac ALL_DISTINCT_MAP_INJ >> simp[] ) >>
     Cases >> simp[] >>
     metis_tac[explode_implode,implode_def] ))
+
+(* Alternative characterisation of VARIANT, and thereby of VSUBST and INST_CORE.
+   Better for evaluation. *)
+
+val vfree_in_def = Define `
+  vfree_in v tm =
+    case tm of
+      Abs bv bod => v <> bv /\ vfree_in v bod
+    | Comb s t => vfree_in v s \/ vfree_in v t
+    | _ => (tm = v)`;
+
+val vfree_in_thm = store_thm("vfree_in_thm",
+  ``!name ty y. (VFREE_IN (Var name ty) y = vfree_in (Var name ty) y)``,
+  ntac 2 gen_tac >> Induct >> simp[VFREE_IN_def,Once vfree_in_def] >>
+  simp[Once vfree_in_def,SimpRHS] >>
+  BasicProvers.CASE_TAC >>
+  simp[Q.SPECL[`Var x1 ty1`,`Var x2 ty2`]vfree_in_def] >>
+  simp[Q.SPECL[`Var x1 ty1`,`Const x2 ty2`]vfree_in_def] >>
+  simp[Q.SPECL[`Var x1 ty1`,`Comb x2 ty2`]vfree_in_def] >>
+  simp[Q.SPECL[`Var x1 ty1`,`Abs x2 ty2`]vfree_in_def] >>
+  METIS_TAC[])
+
+val variant_def = tDefine "variant" `
+  variant avoid v =
+    if EXISTS (vfree_in v) avoid then
+    case v of
+       Var s ty => variant avoid (Var(s ^ (strlit "'")) ty)
+    | _ => v else v`
+  (WF_REL_TAC `measure (\(avoid,v).
+     let n = SUM_SET (BIGUNION (set (MAP (λa. {strlen x + 1 | ∃ty. VFREE_IN (Var x ty) a}) avoid))) in
+       n - (case v of Var x ty => strlen x | _ => 0))` >>
+   gen_tac >> Cases >> rw[strlen_def,strcat_def,explode_implode] >>
+   qsuff_tac`STRLEN s' < n` >- simp[] >>
+   simp[Abbr`n`] >> fs[GSYM vfree_in_thm,EXISTS_MEM] >>
+   match_mp_tac SUM_SET_IN_LT >>
+   qexists_tac`STRLEN s' + 1` >> simp[MEM_MAP,PULL_EXISTS] >>
+   map_every qexists_tac[`e`,`strlit s'`,`ty`] >> simp[] >> rw[] >>
+   qmatch_abbrev_tac`FINITE s` >>
+   `s = IMAGE (λ(x,ty). strlen x + 1) {(x,ty) | VFREE_IN (Var x ty) a}` by (
+     simp[Abbr`s`,pred_setTheory.EXTENSION,PULL_EXISTS,strlen_def] ) >>
+   pop_assum SUBST1_TAC >>
+   match_mp_tac pred_setTheory.IMAGE_FINITE >>
+   simp[])
+
+val variant_ind = fetch "-" "variant_ind"
+
+val variant_vsubst_thm = save_thm("variant_vsubst_thm",prove(
+  ``!xs v x name.
+      (xs = [x]) /\ (v = (Var name ty)) ==>
+      (variant xs (Var name ty) =
+       Var (VARIANT x (explode name) ty) ty)``,
+  REWRITE_TAC [VARIANT_def] \\ HO_MATCH_MP_TAC variant_ind
+  \\ SIMP_TAC std_ss [] \\ REPEAT STRIP_TAC
+  \\ ASM_SIMP_TAC (srw_ss()) [Once variant_def,EXISTS_DEF]
+  \\ MP_TAC (Q.SPECL[`name`,`ty`, `x`] vfree_in_thm) \\ FULL_SIMP_TAC std_ss [] \\ STRIP_TAC
+  \\ FULL_SIMP_TAC (srw_ss()) [EXISTS_DEF]
+  \\ REVERSE IF_CASES_TAC
+  \\ FULL_SIMP_TAC (srw_ss()) [] THEN1
+   (MP_TAC (VARIANT_PRIMES_def |> Q.SPECL [`x`,`explode name`,`ty`])
+    \\ Cases_on `VARIANT_PRIMES x (explode name) ty`
+    THEN1 (FULL_SIMP_TAC (srw_ss()) [rich_listTheory.REPLICATE,mlstringTheory.implode_explode])
+    \\ REPEAT STRIP_TAC \\ POP_ASSUM (MP_TAC o Q.SPEC `0`)
+    \\ FULL_SIMP_TAC (srw_ss()) [rich_listTheory.REPLICATE,mlstringTheory.implode_explode])
+  \\ MP_TAC (VARIANT_PRIMES_def |> Q.SPECL [`x`,`explode name`,`ty`])
+  \\ Cases_on `VARIANT_PRIMES x (explode name) ty`
+  \\ FULL_SIMP_TAC (srw_ss()) [rich_listTheory.REPLICATE,mlstringTheory.implode_explode]
+  \\ REPEAT STRIP_TAC
+  \\ `!m. m < n ==>
+         VFREE_IN (Var (name ^ (implode (REPLICATE (SUC m) #"'"))) ty) x` by ALL_TAC
+  THEN1 (REPEAT STRIP_TAC \\ `SUC m < SUC n` by DECIDE_TAC \\ RES_TAC \\ FULL_SIMP_TAC std_ss [rich_listTheory.REPLICATE_GENLIST]
+         \\ FULL_SIMP_TAC std_ss [mlstringTheory.strcat_def,mlstringTheory.explode_implode])
+  \\ FULL_SIMP_TAC (srw_ss()) [rich_listTheory.REPLICATE_GENLIST,GENLIST_CONS]
+  \\ MP_TAC (VARIANT_PRIMES_def |> Q.SPECL [`x`,`explode (name ^ strlit "'")`,`ty`])
+  \\ FULL_SIMP_TAC std_ss [GSYM APPEND_ASSOC,APPEND,mlstringTheory.strcat_def,mlstringTheory.explode_implode,mlstringTheory.explode_def]
+  \\ Cases_on `VARIANT_PRIMES x (STRCAT (explode name) "'") (ty) = n`
+  \\ FULL_SIMP_TAC std_ss []
+  \\ REPEAT STRIP_TAC
+  \\ `VARIANT_PRIMES x (STRCAT (explode name) "'") ty < n \/
+      n < VARIANT_PRIMES x (STRCAT (explode name) "'") ty` by DECIDE_TAC
+  \\ RES_TAC \\ FULL_SIMP_TAC std_ss [])
+  |> SIMP_RULE std_ss [] |> SPEC_ALL);
+
+val VSUBST_thm = save_thm("VSUBST_thm",
+  REWRITE_RULE[SYM variant_vsubst_thm] VSUBST_def)
+
+val subtract_def = Define `
+  subtract l1 l2 = FILTER (\t. ~(MEM t l2)) l1`;
+
+val insert_def = Define `
+  insert x l = if MEM x l then l else x::l`;
+
+val itlist_def = Define `
+  itlist f l b =
+    case l of
+      [] => b
+    | (h::t) => f h (itlist f t b)`;
+
+val union_def = Define `
+  union l1 l2 = itlist insert l1 l2`;
+
+val MEM_union = store_thm("MEM_union",
+  ``!xs ys x. MEM x (union xs ys) <=> MEM x xs \/ MEM x ys``,
+  Induct \\ FULL_SIMP_TAC std_ss [union_def]
+  \\ ONCE_REWRITE_TAC [itlist_def] \\ SRW_TAC [] [insert_def]
+  \\ METIS_TAC []);
+
+val EXISTS_union = store_thm("EXISTS_union",
+  ``!xs ys. EXISTS P (union xs ys) <=> EXISTS P xs \/ EXISTS P ys``,
+  SIMP_TAC std_ss [EXISTS_MEM,MEM_MAP,MEM_union] \\ METIS_TAC []);
+
+val frees_def = Define `
+  frees tm =
+    case tm of
+      Var _ _ => [tm]
+    | Const _ _ => []
+    | Abs bv bod => subtract (frees bod) [bv]
+    | Comb s t => union (frees s) (frees t)`
+
+val MEM_frees_EQ = store_thm("MEM_frees_EQ",
+  ``!a x. MEM x (frees a) = ?n ty. (x = Var n ty) /\ MEM (Var n ty) (frees a)``,
+  Induct \\ SIMP_TAC (srw_ss()) [Once frees_def,MEM_union]
+  THEN1 (SIMP_TAC (srw_ss()) [Once frees_def,MEM_union])
+  THEN1 (SIMP_TAC (srw_ss()) [Once frees_def,MEM_union])
+  \\ ONCE_REWRITE_TAC [EQ_SYM_EQ]
+  \\ SIMP_TAC (srw_ss()) [Once frees_def,MEM_union] THEN1 (METIS_TAC [])
+  \\ SIMP_TAC (srw_ss()) [subtract_def,MEM_FILTER]
+  \\ REPEAT STRIP_TAC \\ EQ_TAC \\ REPEAT STRIP_TAC \\ METIS_TAC []);
+
+val variant_inst_thm = save_thm("variant_inst_thm",prove(
+  ``!xs v x name a.
+      welltyped a ∧
+      (xs = frees a) /\
+      (v = (Var name ty1)) ==>
+      (variant (frees a) (Var name ty1) =
+       Var (VARIANT a (explode name) ty1) ty1)``,
+  REWRITE_TAC [VARIANT_def] \\ HO_MATCH_MP_TAC variant_ind
+  \\ SIMP_TAC std_ss [] \\ REPEAT STRIP_TAC
+  \\ ASM_SIMP_TAC (srw_ss()) [Once variant_def,EXISTS_DEF]
+  \\ `EXISTS (vfree_in (Var name ty1)) (frees a) =
+      VFREE_IN (Var name ty1) a` by ALL_TAC THEN1
+   (Q.PAT_ASSUM `welltyped a` MP_TAC (* \\ Q.PAT_ASSUM `TYPE defs ty1` MP_TAC *)
+    (* \\ Q.MATCH_ASSUM_RENAME_TAC `STATE defs st` [] *)
+    (* \\ Q.PAT_ASSUM `STATE defs st ` MP_TAC *) \\ REPEAT (POP_ASSUM (K ALL_TAC))
+    \\ Induct_on `a` \\ SIMP_TAC (srw_ss()) [Once frees_def,Once vfree_in_def]
+    THEN1 (REPEAT STRIP_TAC
+      \\ FULL_SIMP_TAC std_ss [EXISTS_union,VFREE_IN_def])
+    \\ REPEAT STRIP_TAC
+    \\ FULL_SIMP_TAC std_ss []
+    \\ BasicProvers.VAR_EQ_TAC
+    \\ FULL_SIMP_TAC std_ss [VFREE_IN_def,WELLTYPED_CLAUSES]
+    \\ FIRST_X_ASSUM (fn th => FULL_SIMP_TAC std_ss [SYM th])
+    \\ FULL_SIMP_TAC (srw_ss()) [EXISTS_MEM,subtract_def,MEM_FILTER,PULL_EXISTS]
+    \\ ONCE_REWRITE_TAC [MEM_frees_EQ]
+    \\ FULL_SIMP_TAC std_ss [term_11,PULL_EXISTS]
+    \\ ONCE_REWRITE_TAC [vfree_in_def] \\ FULL_SIMP_TAC (srw_ss()) []
+    \\ METIS_TAC [])
+  \\ FULL_SIMP_TAC std_ss []
+  \\ REVERSE (Cases_on `VFREE_IN (Var name ty1) a`) THEN1
+   (MP_TAC (VARIANT_PRIMES_def |> Q.SPECL [`a`,`explode name`,`ty1`])
+    \\ Cases_on `VARIANT_PRIMES a (explode name) ty1`
+    THEN1 FULL_SIMP_TAC (srw_ss()) [rich_listTheory.REPLICATE,mlstringTheory.implode_explode]
+    \\ REPEAT STRIP_TAC \\ POP_ASSUM (MP_TAC o Q.SPEC `0`)
+    \\ FULL_SIMP_TAC (srw_ss()) [rich_listTheory.REPLICATE,mlstringTheory.implode_explode])
+  \\ MP_TAC (VARIANT_PRIMES_def |> Q.SPECL [`a`,`explode name`,`ty1`])
+  \\ Cases_on `VARIANT_PRIMES a (explode name) ty1`
+  \\ FULL_SIMP_TAC (srw_ss()) [rich_listTheory.REPLICATE,mlstringTheory.implode_explode]
+  \\ REPEAT STRIP_TAC
+  \\ POP_ASSUM (ASSUME_TAC o Q.GEN `m` o SIMP_RULE std_ss [] o Q.SPEC `SUC m`)
+  \\ MP_TAC (VARIANT_PRIMES_def |> Q.SPECL [`a`,`STRCAT (explode name) "'"`,`ty1`])
+  \\ FULL_SIMP_TAC std_ss [GSYM APPEND_ASSOC,APPEND,mlstringTheory.strcat_def,mlstringTheory.explode_def,mlstringTheory.explode_implode]
+  \\ Q.ABBREV_TAC `k = VARIANT_PRIMES a (STRCAT (explode name) "'") ty1`
+  \\ FULL_SIMP_TAC (srw_ss()) [rich_listTheory.REPLICATE_GENLIST,GENLIST_CONS]
+  \\ Cases_on `k = n` \\ FULL_SIMP_TAC std_ss []
+  \\ REPEAT STRIP_TAC
+  \\ `k < n \/ n < k` by DECIDE_TAC
+  \\ RES_TAC \\ FULL_SIMP_TAC std_ss [])
+  |> SIMP_RULE std_ss [] |> SPEC_ALL);
+
+val INST_CORE_Abs_thm = store_thm("INST_CORE_Abs_thm",
+  ``∀v t env tyin. welltyped (Abs v t) ⇒
+   INST_CORE env tyin (Abs v t) =
+   (let (x,ty) = dest_var v in
+    let ty' = TYPE_SUBST tyin ty in
+    let v' = Var x ty' in
+    let env' = (v,v')::env in
+    let tres = INST_CORE env' tyin t
+    in
+      if IS_RESULT tres then Result (Abs v' (RESULT tres))
+      else
+        (let w = CLASH tres
+         in
+           if w ≠ v' then tres
+           else
+             (let (x',_) =
+               dest_var (variant (frees (RESULT (INST_CORE [] tyin t))) (Var x ty'))
+              in
+              let t' = VSUBST [(Var x' ty,Var x ty)] t in
+              let env'' = (Var x' ty,Var x' ty')::env in
+              let tres' = INST_CORE env'' tyin t'
+              in
+                if IS_RESULT tres' then
+                  Result (Abs (Var x' ty') (RESULT tres'))
+                else tres')))``,
+  rw[] >> simp[Once INST_CORE_def] >> rw[] >>
+  unabbrev_all_tac >> fs[] >>
+  rfs[GSYM INST_def] >>
+  imp_res_tac INST_WELLTYPED >>
+  fs[variant_inst_thm] >> rw[] >> fs[])
 
 (* provable terms are ok and of type bool *)
 
